#! https://zhuanlan.zhihu.com/p/539856504

---
- 文献：[前苏下](https://book.douban.com/subject/10828594/)
- 首发：[Zydragon-x's Blog](https://zydragon-x.github.io/2022/07/10/problems/)


## 2022.7.10

【题】：试证明$\displaystyle\sum_{n=1}^{\infty} \frac{(-1)^{\left[2^{n} x\right]}}{2^{n}}=1+2[x]-2x,x\geq 0$. $\blacktriangleright$ 

$\blacktriangleleft$  设$x=(\overline{a_{k}a_{k-1}\cdots a_0 .b_1b_2\cdots })_2$为$x$的标准二进制表示,则对于$\forall n\in\mathbb{N_{+}}$,有

$[2^nx]=(\overline{a_{k}a_{k-1}\cdots a_0 b_1b_2\cdots b_n})_2\equiv b_n(\mod2)$,

考虑到$b_n\in\{0,1\}$,故必有$(-1)^{[2^nx]}=(-1)^{b_n}=1-2b_n$,从而

$\begin{aligned} \displaystyle\sum_{n=1}^{\infty} \frac{(-1)^{\left[2^{n} x\right]}}{2^{n}}
&=\displaystyle\sum_{n=1}^{\infty} \frac{1-2b_n}{2^{n}} 
=\displaystyle\sum_{n=1}^{\infty}\frac{1}{2^n}-2\displaystyle\sum_{n=1}^{\infty} \frac{b_n}{2^n} \\
&=1-2(\overline{0.b_1 b_2\cdots})_2
=1-2(x-[x])=1+2[x]-2x .\blacksquare
\end{aligned}$ 


## 2022.7.11
 

